CoqOfRust/examples/default/examples/error_handling/combinators_map.v
@@ -108,7 +108,7 @@ Section Impl_core_fmt_Debug_for_combinators_map_Peeled_t.
     let* α3 : M.Val (ref combinators_map.Food.t) :=
       M.alloc (borrow (deref α2).["0"]) in
     let* α4 : M.Val (ref (ref combinators_map.Food.t)) := M.alloc (borrow α3) in
-    let* α5 : ref dynamic := M.read (pointer_coercion "Unsize" α4) in
+    let* α5 : ref _ (* dyn *) := M.read (pointer_coercion "Unsize" α4) in
     M.call (core.fmt.Formatter.t::["debug_tuple_field1_finish"] α0 α1 α5).
   
   Global Instance AssociatedFunction_fmt : Notations.DoubleColon Self "fmt" := {
@@ -153,7 +153,7 @@ Section Impl_core_fmt_Debug_for_combinators_map_Chopped_t.
     let* α3 : M.Val (ref combinators_map.Food.t) :=
       M.alloc (borrow (deref α2).["0"]) in
     let* α4 : M.Val (ref (ref combinators_map.Food.t)) := M.alloc (borrow α3) in
-    let* α5 : ref dynamic := M.read (pointer_coercion "Unsize" α4) in
+    let* α5 : ref _ (* dyn *) := M.read (pointer_coercion "Unsize" α4) in
     M.call (core.fmt.Formatter.t::["debug_tuple_field1_finish"] α0 α1 α5).
   
   Global Instance AssociatedFunction_fmt : Notations.DoubleColon Self "fmt" := {
@@ -198,7 +198,7 @@ Section Impl_core_fmt_Debug_for_combinators_map_Cooked_t.
     let* α3 : M.Val (ref combinators_map.Food.t) :=
       M.alloc (borrow (deref α2).["0"]) in
     let* α4 : M.Val (ref (ref combinators_map.Food.t)) := M.alloc (borrow α3) in
-    let* α5 : ref dynamic := M.read (pointer_coercion "Unsize" α4) in
+    let* α5 : ref _ (* dyn *) := M.read (pointer_coercion "Unsize" α4) in
     M.call (core.fmt.Formatter.t::["debug_tuple_field1_finish"] α0 α1 α5).
   
   Global Instance AssociatedFunction_fmt : Notations.DoubleColon Self "fmt" := {
