CoqOfRust/examples/default/examples/error_handling/other_uses_of_question_mark.v
@@ -160,13 +160,15 @@ Definition double_first
                 let* α1 :
                     core.result.Result.t
                       i32.t
-                      (alloc.boxed.Box.t dynamic alloc.alloc.Global.t) :=
+                      (alloc.boxed.Box.t _ (* dyn *) alloc.alloc.Global.t) :=
                   M.call
                     ((core.ops.try_trait.FromResidual.from_residual
                         (Self :=
                           core.result.Result.t
                             i32.t
-                            (alloc.boxed.Box.t dynamic alloc.alloc.Global.t))
+                            (alloc.boxed.Box.t
+                              _ (* dyn *)
+                              alloc.alloc.Global.t))
                         (Trait := ltac:(refine _)))
                       α0) in
                 let* α2 : M.Val never.t := return_ α1 in
@@ -231,13 +233,15 @@ Definition double_first
                 let* α1 :
                     core.result.Result.t
                       i32.t
-                      (alloc.boxed.Box.t dynamic alloc.alloc.Global.t) :=
+                      (alloc.boxed.Box.t _ (* dyn *) alloc.alloc.Global.t) :=
                   M.call
                     ((core.ops.try_trait.FromResidual.from_residual
                         (Self :=
                           core.result.Result.t
                             i32.t
-                            (alloc.boxed.Box.t dynamic alloc.alloc.Global.t))
+                            (alloc.boxed.Box.t
+                              _ (* dyn *)
+                              alloc.alloc.Global.t))
                         (Trait := ltac:(refine _)))
                       α0) in
                 let* α2 : M.Val never.t := return_ α1 in
@@ -265,7 +269,7 @@ Definition double_first
         M.Val
           (core.result.Result.t
             i32.t
-            (alloc.boxed.Box.t dynamic alloc.alloc.Global.t)) :=
+            (alloc.boxed.Box.t _ (* dyn *) alloc.alloc.Global.t)) :=
       M.alloc (core.result.Result.Ok α1) in
     M.read α0).
 
@@ -399,7 +403,7 @@ Definition main : M unit :=
     let* α1 :
         core.result.Result.t
           i32.t
-          (alloc.boxed.Box.t dynamic alloc.alloc.Global.t) :=
+          (alloc.boxed.Box.t _ (* dyn *) alloc.alloc.Global.t) :=
       M.call (other_uses_of_question_mark.double_first α0) in
     let* α2 : unit := M.call (other_uses_of_question_mark.print α1) in
     M.alloc α2 in
@@ -409,7 +413,7 @@ Definition main : M unit :=
     let* α1 :
         core.result.Result.t
           i32.t
-          (alloc.boxed.Box.t dynamic alloc.alloc.Global.t) :=
+          (alloc.boxed.Box.t _ (* dyn *) alloc.alloc.Global.t) :=
       M.call (other_uses_of_question_mark.double_first α0) in
     let* α2 : unit := M.call (other_uses_of_question_mark.print α1) in
     M.alloc α2 in
@@ -419,7 +423,7 @@ Definition main : M unit :=
     let* α1 :
         core.result.Result.t
           i32.t
-          (alloc.boxed.Box.t dynamic alloc.alloc.Global.t) :=
+          (alloc.boxed.Box.t _ (* dyn *) alloc.alloc.Global.t) :=
       M.call (other_uses_of_question_mark.double_first α0) in
     let* α2 : unit := M.call (other_uses_of_question_mark.print α1) in
     M.alloc α2 in
