CoqOfRust/examples/default/examples/scoping_rules/scoping_rules_ownership_and_rules_partial_moves.v
@@ -196,7 +196,7 @@ Section Impl_core_fmt_Debug_for_scoping_rules_ownership_and_rules_partial_moves_
       M.read self in
     let* α4 : M.Val (ref alloc.string.String.t) :=
       M.alloc (borrow (deref α3).["name"]) in
-    let* α5 : ref dynamic := M.read (pointer_coercion "Unsize" α4) in
+    let* α5 : ref _ (* dyn *) := M.read (pointer_coercion "Unsize" α4) in
     let* α6 : ref str.t := M.read (mk_str "age") in
     let* α7 :
         ref scoping_rules_ownership_and_rules_partial_moves.main.Person.t :=
@@ -205,7 +205,7 @@ Section Impl_core_fmt_Debug_for_scoping_rules_ownership_and_rules_partial_moves_
       M.alloc (borrow (deref α7).["age"]) in
     let* α9 : M.Val (ref (ref (alloc.boxed.Box.t u8.t alloc.alloc.Global.t))) :=
       M.alloc (borrow α8) in
-    let* α10 : ref dynamic := M.read (pointer_coercion "Unsize" α9) in
+    let* α10 : ref _ (* dyn *) := M.read (pointer_coercion "Unsize" α9) in
     M.call
       (core.fmt.Formatter.t::["debug_struct_field2_finish"] α0 α1 α2 α5 α6 α10).
   
