CoqOfRust/examples/default/examples/std_misc/channels.v
@@ -249,7 +249,7 @@ Definition main : M unit :=
                     alloc.alloc.Global.t) :=
               let* α0 : ref i32.t := M.read channels.NTHREADS in
               let* α1 : i32.t := M.read (deref α0) in
-              let* α2 : usize.t := cast α1 in
+              let* α2 : usize.t := M.cast α1 in
               let* α3 :
                   alloc.vec.Vec.t
                     (core.result.Result.t i32.t std.sync.mpsc.RecvError.t)
@@ -411,7 +411,7 @@ Definition main : M unit :=
                                         core.result.Result.t
                                           unit
                                           (alloc.boxed.Box.t
-                                            dynamic
+                                            _ (* dyn *)
                                             alloc.alloc.Global.t) :=
                                       M.call
                                         ((std.thread.JoinHandle.t
@@ -426,7 +426,7 @@ Definition main : M unit :=
                                         ((core.result.Result.t
                                               unit
                                               (alloc.boxed.Box.t
-                                                dynamic
+                                                _ (* dyn *)
                                                 alloc.alloc.Global.t))::["expect"]
                                           α1
                                           α2) in
